<exercise checkit-seed="0008" checkit-slug="DiffProdQuot" checkit-title="Product/Quotient Rule">
    <statement>
        <p>
            Demonstrate and explain how to find the derivative of the following functions.
            Be sure to explicitly denote which derivative rules (product, quotient, sum and difference, etc.) you are using in your work.
        </p>
        <ol>
            <li><me>f(w)= -{\left(6 \, w^{2} - 2 \, w - 1\right)} \log\left(w\right)</me></li>
            <li><me>h(w)= -\frac{2 \, {\left(w^{2} + 3 \, w + 1\right)}}{w^{4}}</me></li>
            <li><me>g(y)= -\frac{e^{y}}{3 \, y^{2} + 3 \, y - 5}</me></li>
        </ol>
    </statement>
    <answer>
        <ol>
            <li><me>f' (w)= -2 \, {\left(6 \, w - 1\right)} \log\left(w\right) - \frac{6 \, w^{2} - 2 \, w - 1}{w}</me></li>
            <li><me>h' (w)= \frac{2 \, {\left(2 \, w^{2} + 9 \, w + 4\right)}}{w^{5}}</me></li>
            <li><me>g' (y)= -\frac{e^{y}}{3 \, y^{2} + 3 \, y - 5} + \frac{3 \, {\left(2 \, y + 1\right)} e^{y}}{{\left(3 \, y^{2} + 3 \, y - 5\right)}^{2}}</me></li>
        </ol>
    </answer>
</exercise>
