<exercise checkit-seed="0000" checkit-slug="DiffStrategy" checkit-title="Differentiation strategy">
    <statement>
        <p>
            Demonstrate and explain how to find the derivative of the following functions.
            Be sure to explicitly denote which derivative rules (constant multiple, sum and difference, etc.) you are using in your work.
        </p>
        <ol>
            <!-- <li> <me>() = \left(  \right)^ </me></li>
            <li><me>() =   </me></li>
            <li><me>() = </me></li> -->
                    <li><p><me>f(x) = \sqrt{\cos\left(3 \, x^{3} + 2\right)}</me></p></li>
                    <li><p><me>
                        g(y) = \left( \frac{2 \, y^{3} + 1}{y^{2} - 2} \right)^{ 4 }
                    </me></p></li>
                    <li><p><me>h(w) = {\left(5 \, w^{3} - 7 \, w\right)}^{6} w^{\frac{1}{3}}</me></p></li>
        </ol>
        

    </statement>
    <answer>
        <ol>
            <!-- <li><me>&apos;() =   \left(  \right)^ \left(  \right) </me></li>
            <li><me>&apos;() =  </me></li>
            <li><me>&apos;() =  </me></li> -->
                    <li><p><me>f ' (x) = -\frac{9 \, x^{2} \sin\left(3 \, x^{3} + 2\right)}{2 \, \sqrt{\cos\left(3 \, x^{3} + 2\right)}}</me></p></li>
                    <li><p><me>
                        g ' (y) = 4
                        \left( \frac{2 \, y^{3} + 1}{y^{2} - 2} \right)^{ 3 }
                        \left( \frac{6 \, y^{2}}{y^{2} - 2} - \frac{2 \, {\left(2 \, y^{3} + 1\right)} y}{{\left(y^{2} - 2\right)}^{2}} \right)
                    </me></p></li>
                    <li><p><me>h ' (w) = 6 \, {\left(5 \, w^{3} - 7 \, w\right)}^{5} {\left(15 \, w^{2} - 7\right)} w^{\frac{1}{3}} + \frac{{\left(5 \, w^{3} - 7 \, w\right)}^{6}}{3 \, w^{\frac{2}{3}}}</me></p></li>
        </ol>

    </answer>
</exercise>
